More pearlite updates, and some statements about piggybank

examples/piggybank/src/piggybank.rs
@@ -69,6 +69,7 @@ pub fn piggy_init_hacspec() -> PiggyBankStateHacspec {
 
 #[cfg(feature = "hacspec")]
 #[init(contract = "PiggyBank")]
+#[ensures(result == (ctx, PiggyBankStateHacspec::Intact))]
 pub fn piggy_init(ctx : Context) -> (Context, PiggyBankStateHacspec) { // , actions
     // Always succeeds
     (ctx, piggy_init_hacspec())
@@ -149,6 +150,15 @@ fn coerce_rust_to_hacspec_context(ctx: &impl HasReceiveContext) -> Result<Contex
 
 type PiggySmashResult = Result<PiggyBankStateHacspec, SmashError>;
 
+#[ensures(!(state == PiggyBankStateHacspec::Intact) ==> result == PiggySmashResult::Err(SmashError::AlreadySmashed))]
+#[ensures(forall<owner : UserAddress>
+          forall<sender : UserAddress>
+          forall<balance : u64>
+          forall<metadata : u64>
+          ctx == Context(owner, sender, balance, metadata) ==>
+          !(owner == sender) ==>
+          result == PiggySmashResult::Err(SmashError::NotOwner)
+)]
 fn piggy_smash_hacspec(ctx: Context, state: PiggyBankStateHacspec) -> PiggySmashResult {
     // Get the contract owner, i.e. the account who initialized the contract.
     let Context(owner, sender, _balance, _metadata) = ctx;
